lib: add notM and notM_wp
Signed-off-by: Michael McInerney <michael.mcinerney@proofcraft.systems>

lib/Monads/NonDetMonad.thy
@@ -606,6 +606,9 @@ notation (output)
 
 section "Combinators that have conditions with side effects"
 
+definition notM :: "('s, bool) nondet_monad \<Rightarrow> ('s, bool) nondet_monad" where
+  "notM m = do c \<leftarrow> m; return (\<not> c) od"
+
 definition
   whileM :: "('s, bool) nondet_monad \<Rightarrow> ('s, 'a) nondet_monad \<Rightarrow> ('s, unit) nondet_monad" where
   "whileM C B \<equiv> do
